More work on proof

Models/Interleaving.thy
@@ -259,24 +259,8 @@ lemma lmap_unl_to_lmap_Inl: "(\<forall>x\<in>lset xs. is_left x) \<Longrightarro
 lemma lmap_unr_to_lmap_Inr: "(\<forall>x\<in>lset xs. is_right x) \<Longrightarrow> lmap unr xs = ys \<longleftrightarrow> xs = lmap Inr ys"
   sorry
 
-datatype element_spec = Nth_Left nat | Nth_Right nat
-
-definition compare_pos :: "element_spec \<Rightarrow> element_spec \<Rightarrow> ('a + 'b) llist \<Rightarrow> bool" (infix "\<lless>" 90) where
-  "x \<lless> y = (\<lambda>xs. undefined)"
-
-lemma compare_pos_irrefl: "\<not> (x \<lless> x) xs"
-  sorry
-
-lemma compare_pos_total: "(x \<lless> y) xs \<or> (y \<lless> x) xs"
-  sorry
-
-lemma compare_pos_trans: "(x \<lless> y) xs \<Longrightarrow> (y \<lless> z) xs \<Longrightarrow> (x \<lless> z) xs"
-  sorry
-
 lemma llength_strict_le: "lprefix xs ys \<Longrightarrow> xs \<noteq> ys \<Longrightarrow> llength xs < llength ys"
   by (metis le_llist_conv_lprefix less_llist_conv_lstrict_prefix lstrict_prefix_llength_less order.not_eq_order_implies_strict)
-
-lemma "lnth (xs \<frown> LCons x xs \<triangleright> t \<triangleleft> ys) (llength (ltakeLeft (llength xs) t)) = x"
 
 lemma lprefix_ltakeLeft_nat: "lprefix (ltakeLeft_nat n t) (ltakeLeft_nat (Suc n) t)"
   apply (induct n arbitrary: t)
@@ -296,6 +280,24 @@ lemma lprefix_ltakeLeft: "lprefix (ltakeLeft n t) (ltakeLeft (eSuc n) t)"
   apply (simp only: eSuc_enat ltakeLeft.simps)
   by (metis lprefix_ltakeLeft_nat)
 
+lemma lprefix_ltakeRight_nat: "lprefix (ltakeRight_nat n t) (ltakeRight_nat (Suc n) t)"
+  apply (induct n arbitrary: t)
+  apply simp
+  apply (metis lprefix_lappend)
+  apply auto
+  apply (subgoal_tac "ldropWhile is_left t = LNil \<or> (\<exists>x xs'. ldropWhile is_left t = LCons x xs')")
+  apply (erule disjE)
+  apply simp
+  apply (erule exE)+
+  apply simp
+  by (metis neq_LNil_conv)
+
+lemma lprefix_ltakeRight: "lprefix (ltakeRight n t) (ltakeRight (eSuc n) t)"
+  apply (cases n)
+  apply auto
+  apply (simp only: eSuc_enat ltakeLeft.simps)
+  by (metis lprefix_ltakeRight_nat ltakeRight.simps(2))  
+
 lemma lprefix_not_itself: "lfinite xs \<Longrightarrow> ys \<noteq> LNil \<Longrightarrow> xs \<noteq> xs \<frown> ys"
   by (metis lstrict_prefix_def lstrict_prefix_lappend_conv)
 
@@ -305,8 +307,35 @@ lemma postfix_not_equal: "lfinite xs \<Longrightarrow> ys \<noteq> zs \<Longrigh
 lemma tail_not_equal: "xs \<noteq> ys \<Longrightarrow> x # xs \<noteq> x # ys"
   by (metis llist.inject)
 
-lemma ldropWhile_cases: "ldropWhile P xs = LNil \<or> (\<exists>y ys. ldropWhile P xs = LCons y ys \<and> P y)"
-  sorry
+lemma lset_split_eq: "x \<in> lset xs \<longleftrightarrow> (\<exists>ys zs. xs = ys \<frown> (x # zs) \<and> lfinite ys)"
+  apply default
+  apply (metis split_llist)
+  by (metis in_lset_lappend_iff lhd_LCons lhd_in_lset llist.distinct(1))
+
+lemma ldropWhile_cases: "ldropWhile P xs = LNil \<or> (\<exists>y ys. ldropWhile P xs = LCons y ys \<and> \<not> P y)"
+  apply (cases "\<forall>x\<in>lset xs. P x")
+  apply simp
+  apply (intro disjI2)
+  apply auto
+  apply (drule split_llist)
+  apply (erule exE)+
+  apply (erule conjE)
+  apply (rotate_tac 1)
+  apply (erule ssubst)
+  apply (erule lfinite_induct)
+  apply (rule_tac x = x in exI)
+  apply simp
+  apply (erule exE)
+  apply (erule conjE)
+  apply (erule exE)
+  apply (subgoal_tac "P xa \<or> \<not> P xa")
+  apply (erule disjE)
+  apply simp
+  apply simp
+  by simp
+
+lemma [simp]: "lfilter is_left (ltakeWhile is_right t) = LNil"
+  by (metis Not_is_left lfilter_ltakeWhile)
 
 lemma ltakeLeft_nat_not_equal_Suc: "enat n < llength (\<ll> t) \<Longrightarrow> ltakeLeft_nat n t \<noteq> ltakeLeft_nat (Suc n) t"
   apply (induct n arbitrary: t)
@@ -321,7 +350,13 @@ lemma ltakeLeft_nat_not_equal_Suc: "enat n < llength (\<ll> t) \<Longrightarrow>
   apply simp
   apply simp
   apply (metis lappend_inf lappend_ltakeWhile_ldropWhile ldropWhile_K_True ldropWhile_eq_ldrop llist.discI ltakeWhile_K_True)
-  apply (metis ldropWhile_LCons ldropWhile_cases llist.distinct(1) lnth_0 not_is_left)
+  apply (subgoal_tac "ldropWhile is_right t = LNil \<or> (\<exists>y ys. ldropWhile is_right t = LCons y ys \<and> \<not> is_right y)")
+  apply (erule disjE)
+  apply simp
+  apply (erule exE)+
+  apply simp
+  apply (metis is_right.simps(1) not_is_right obj_sumE)
+  apply (rule ldropWhile_cases)
   apply (simp add: lefts_def)
   apply (subgoal_tac "ldropWhile is_right t = LNil \<or> (\<exists>x xs'. ldropWhile is_right t = LCons (Inl x) xs')")
   apply (erule disjE)
@@ -329,7 +364,13 @@ lemma ltakeLeft_nat_not_equal_Suc: "enat n < llength (\<ll> t) \<Longrightarrow>
   apply (erule exE)+
   apply simp
   defer
-  apply (metis ldropWhile_LCons ldropWhile_cases llist.distinct(1) lnth_0 not_is_left)
+  apply (subgoal_tac "ldropWhile is_right t = LNil \<or> (\<exists>y ys. ldropWhile is_right t = LCons y ys \<and> \<not> is_right y)")
+  apply (erule disjE)
+  apply simp
+  apply (erule exE)+
+  apply simp
+  apply (metis is_right.simps(1) not_is_right obj_sumE)
+  apply (rule ldropWhile_cases)
   apply (subgoal_tac "lfinite (ltakeWhile is_right t)")
   prefer 2
   apply (metis lappend_inf lappend_ltakeWhile_ldropWhile ldropWhile_eq_ldrop ldrop_eq_LConsD less_imp_not_eq)
@@ -340,18 +381,112 @@ lemma ltakeLeft_nat_not_equal_Suc: "enat n < llength (\<ll> t) \<Longrightarrow>
   apply metis
   apply (subgoal_tac "enat (Suc n) < llength (lfilter is_left (ltakeWhile is_right t \<frown> ldropWhile is_right t))")
   apply simp
-  apply (metis is_right.simps(2) ldropWhile_cases llist.distinct(1) llist.inject)
+  apply (metis Suc_ile_eq)
   by (metis lappend_ltakeWhile_ldropWhile)
+
+lemma lmap_swap_n_eq: "xs \<noteq> ys \<Longrightarrow> lmap swap xs \<noteq> lmap swap ys"
+  by (metis lappend_ltakeRight_ldropRight ldropRight_to_ldropLeft ltakeRight_to_ltakeLeft) 
+
+lemma lmap_swap_swap [simp]: "lmap swap (lmap swap xs) = xs"
+  by (metis lappend_ltakeLeft_ldropLeft lappend_ltakeRight_ldropRight ldropLeft_to_ldropRight lmap_lappend_distrib ltakeLeft_to_ltakeRight)
+
+lemma lefts_lmap_swap: "\<ll> (lmap swap xs) = \<rr> xs"
+  apply (simp add: lefts_def rights_def)
+  by (metis is_left_swap lfilter_lmap lmap.compositionality unl_swap)
+
+lemma ltakeRight_nat_not_equal_Suc: "enat n < llength (\<rr> t) \<Longrightarrow> ltakeRight_nat n t \<noteq> ltakeRight_nat (Suc n) t"
+  apply (subgoal_tac "t = lmap swap (lmap swap t)")
+  apply (rotate_tac 1)
+  apply (erule ssubst)
+  apply (subst ltakeRight_nat_to_ltakeLeft_nat)
+  apply (subst ltakeRight_nat_to_ltakeLeft_nat)
+  apply (rule lmap_swap_n_eq)
+  apply (simp only: lmap_swap_swap)
+  apply (rule ltakeLeft_nat_not_equal_Suc)
+  apply (metis lefts_lmap_swap)
+  by simp
 
 lemma ltakeLeft_not_equal_Suc: "n < llength (\<ll> t) \<Longrightarrow> ltakeLeft n t \<noteq> ltakeLeft (eSuc n) t"
   apply (cases n)
   apply auto
   by (metis eSuc_enat ltakeLeft.simps(2) ltakeLeft_nat_not_equal_Suc)
 
-lemma
+lemma ltakeRight_not_equal_Suc: "n < llength (\<rr> t) \<Longrightarrow> ltakeRight n t \<noteq> ltakeRight (eSuc n) t"
+  apply (cases n)
+  apply auto
+  by (metis eSuc_enat ltakeRight.simps(2) ltakeRight_nat_not_equal_Suc)
+
+lemma "t \<noteq> LNil \<longleftrightarrow> llength (ltakeWhile is_right t) \<noteq> llength (ltakeWhile is_left t)"
+  apply (cases t)
+  apply simp
+  apply simp
+  apply auto
+  by (metis not_is_right)
+
+lemma [simp]: "\<up> \<infinity> xs = xs"
+  by (metis lappend_LNil2 lappend_ltake_ldrop ldrop.simps(2))
+
+lemma non_finite_append: "ys \<noteq> LNil \<Longrightarrow> xs \<frown> ys = xs \<Longrightarrow> \<not> lfinite xs"
+  apply (rule classical)
+  apply simp
+  apply (rotate_tac 2)
+  apply (induct rule: lfinite_induct)
+  apply simp
+  by simp
+
+lemma ltake_lappend_llength_enat': "\<up> (enat i) (xs \<frown> ys) = \<up> (enat i) xs \<Longrightarrow> ys \<noteq> LNil \<longrightarrow> enat i \<le> llength xs"
+  apply (induct i arbitrary: xs)
+  apply (simp add: enat_0)
+  apply (subgoal_tac "(\<exists>x' xs'. xs = x' # xs') \<or> xs = LNil")
+  apply (erule disjE)
+  apply (erule exE)+
+  apply (simp add: eSuc_enat[symmetric])
+  apply simp
+  apply (simp add: eSuc_enat[symmetric])
+  by (metis neq_LNil_conv)
+
+lemma ltake_lappend_llength': "\<up> n (xs \<frown> ys) = \<up> n xs \<Longrightarrow> ys \<noteq> LNil \<longrightarrow> n \<le> llength xs"
+  apply (cases "n = \<infinity>")
+  apply simp
+  apply (metis llength_eq_infty_conv_lfinite lprefix_not_itself)
+  apply simp
+  apply (erule exE)
+  apply simp
+  by (metis ltake_lappend_llength_enat')
+
+lemma ltake_lappend_llength: "ys \<noteq> LNil \<Longrightarrow> \<up> n (xs \<frown> ys) = \<up> n xs \<longleftrightarrow> n \<le> llength xs"
+  by (metis ltake_lappend1 ltake_lappend_llength')
+
+lemma just_lefts: "Valid xs t LNil \<Longrightarrow> xs \<triangleright> t \<triangleleft> LNil = lmap Inl xs"
+  sorry
+
+lemma just_rights: "Valid LNil t ys \<Longrightarrow> LNil \<triangleright> t \<triangleleft> ys = lmap Inr ys"
+  sorry
+
+lemma analyse_interleavings:
   assumes "Valid (xs \<frown> (x\<^sub>1 # x\<^sub>2 # xs')) t (ys \<frown> (y\<^sub>1 # y\<^sub>2 # ys'))"
-  and "lfinite xs"
-  shows "xs \<frown> (x\<^sub>1 # x\<^sub>2 # xs') \<triangleright> t \<triangleleft> ys \<frown> (y\<^sub>1 # y\<^sub>2 # ys') = Z" (is "?lhs = ?rhs")
+
+  and "lfinite xs" and "lfinite ys"
+
+  and "\<And>xs\<^sub>1' xs\<^sub>2' xs\<^sub>3' t\<^sub>1 t\<^sub>2 t\<^sub>3 ys\<^sub>1 ys\<^sub>2 ys\<^sub>3.
+    Valid xs t\<^sub>1 ys\<^sub>1 \<Longrightarrow> Valid xs\<^sub>1' t\<^sub>2 ys\<^sub>3 \<Longrightarrow> Valid xs\<^sub>3' t\<^sub>3 ys' \<Longrightarrow>
+    xs' = xs\<^sub>1' \<frown> xs\<^sub>2' \<frown> xs\<^sub>3' \<Longrightarrow>
+    ys = ys\<^sub>1 \<frown> ys\<^sub>2 \<frown> ys\<^sub>3 \<Longrightarrow>
+    P ((xs \<triangleright> t\<^sub>1 \<triangleleft> ys\<^sub>1) \<frown> (Inl x\<^sub>1 # LNil) \<frown> lmap Inr ys\<^sub>2 \<frown> (Inl x\<^sub>2 # LNil) \<frown> (xs\<^sub>1' \<triangleright> t\<^sub>2 \<triangleleft> ys\<^sub>3) \<frown>  (Inr y\<^sub>1 # LNil) \<frown> lmap Inl xs\<^sub>2' \<frown> (Inr y\<^sub>2 # LNil) \<frown> (xs\<^sub>3' \<triangleright> t\<^sub>3 \<triangleleft> ys'))"
+
+  and "\<And>xs\<^sub>1' xs\<^sub>2' t\<^sub>1 t\<^sub>2 ys\<^sub>1 ys\<^sub>2.
+    Valid xs t\<^sub>1 ys\<^sub>1 \<Longrightarrow> Valid xs\<^sub>2' t\<^sub>2 ys' \<Longrightarrow>
+    xs' = xs\<^sub>1' \<frown> xs\<^sub>2' \<Longrightarrow>
+    ys = ys\<^sub>1 \<frown> ys\<^sub>2 \<Longrightarrow>
+    P ((xs \<triangleright> t\<^sub>1 \<triangleleft> ys\<^sub>1) \<frown> (Inl x\<^sub>1 # LNil) \<frown> lmap Inr ys\<^sub>2 \<frown> (Inr y\<^sub>1 # LNil) \<frown> (Inl x\<^sub>2 # LNil) \<frown> lmap Inl xs\<^sub>1' \<frown> (Inr y\<^sub>2 # LNil) \<frown> (xs\<^sub>2' \<triangleright> t\<^sub>2 \<triangleleft> ys'))"
+
+  and "\<And>t\<^sub>1 t\<^sub>2 ys\<^sub>1 ys\<^sub>2 ys\<^sub>1' ys\<^sub>2'.
+    Valid xs t\<^sub>1 ys\<^sub>1 \<Longrightarrow> Valid xs' t\<^sub>2 ys\<^sub>2' \<Longrightarrow>
+    ys = ys\<^sub>1 \<frown> ys\<^sub>2 \<Longrightarrow>
+    ys' = ys\<^sub>1' \<frown> ys\<^sub>2' \<Longrightarrow>
+    P ((xs \<triangleright> t\<^sub>1 \<triangleleft> ys\<^sub>1) \<frown> (Inl x\<^sub>1 # LNil) \<frown> lmap Inr ys\<^sub>2 \<frown> (Inr y\<^sub>1 # LNil) \<frown> (Inr y\<^sub>2 # LNil) \<frown> lmap Inr ys\<^sub>1' \<frown> (Inr x\<^sub>2 # LNil) \<frown> (xs' \<triangleright> t\<^sub>2 \<triangleleft> ys\<^sub>2'))"
+
+  shows "P (xs \<frown> (x\<^sub>1 # x\<^sub>2 # xs') \<triangleright> t \<triangleleft> ys \<frown> (y\<^sub>1 # y\<^sub>2 # ys'))"
 proof -
   def px\<^sub>1 \<equiv> "llength (ltakeLeft (llength xs) t)"
   def px\<^sub>2 \<equiv> "llength (ltakeLeft (eSuc (llength xs)) t)"
@@ -369,18 +504,737 @@ proof -
   def py\<^sub>2 \<equiv> "llength (ltakeRight (eSuc (llength ys)) t)"
 
   have "py\<^sub>1 < py\<^sub>2"
-    sorry (* Symmetric to above *)
+    apply (simp add: py\<^sub>1_def py\<^sub>2_def)
+    apply (rule llength_strict_le)
+    apply (metis lprefix_ltakeRight)
+    apply (rule ltakeRight_not_equal_Suc)
+    using assms(1)
+    apply (simp add: Valid_def)
+    by (metis assms(3) lfinite_conv_llength_enat)
 
-  have "?lhs = (xs \<triangleright> ltakeLeft (llength xs) t \<triangleleft> \<up> (llength (\<rr> (ltakeLeft (llength xs) t))) (ys \<frown> (y\<^sub>1 # y\<^sub>2 # ys'))) \<frown>
-               (x\<^sub>1 # x\<^sub>2 # xs' \<triangleright> ldropLeft (llength xs) t \<triangleleft> \<down> (llength (\<rr> (ltakeLeft (llength xs) t))) (ys \<frown> (y\<^sub>1 # y\<^sub>2 # ys')))"
-    by (simp only: interleave_left_lappend[OF assms(1) assms(2)])
+  have "px\<^sub>1 \<noteq> py\<^sub>1"
+    apply (simp add: px\<^sub>1_def py\<^sub>1_def)
+    sorry
 
-  have split_Valid1:
-    "Valid xs (ltakeLeft (llength xs) t) (\<up> (llength (\<rr> (ltakeLeft (llength xs) t))) (ys \<frown> (y\<^sub>1 # y\<^sub>2 # ys')))"
-    by (simp only: interleave_left_lappend[OF assms(1) assms(2)])
+  have "px\<^sub>2 \<noteq> py\<^sub>2"
+    sorry
 
-  have split_Valid2:
-    "Valid (x\<^sub>1 # x\<^sub>2 # xs') (ldropLeft (llength xs) t) (\<down> (llength (\<rr> (ltakeLeft (llength xs) t))) (ys \<frown> (y\<^sub>1 # y\<^sub>2 # ys')))"
-    by (simp only: interleave_left_lappend[OF assms(1) assms(2)])
+  have "px\<^sub>1 \<noteq> py\<^sub>2"
+    sorry
 
+  have "px\<^sub>2 \<noteq> py\<^sub>1"
+    sorry
+
+  have "(px\<^sub>1 < px\<^sub>2 \<and> px\<^sub>2 < py\<^sub>1 \<and> py\<^sub>1 < py\<^sub>2) \<or>
+        (px\<^sub>1 < py\<^sub>1 \<and> py\<^sub>1 < px\<^sub>2 \<and> px\<^sub>2 < py\<^sub>2) \<or>
+        (px\<^sub>1 < py\<^sub>1 \<and> py\<^sub>1 < py\<^sub>2 \<and> py\<^sub>2 < px\<^sub>2) \<or>
+        (py\<^sub>1 < py\<^sub>2 \<and> py\<^sub>2 < px\<^sub>1 \<and> px\<^sub>1 < px\<^sub>2) \<or>
+        (py\<^sub>1 < px\<^sub>1 \<and> px\<^sub>1 < py\<^sub>2 \<and> py\<^sub>2 < px\<^sub>2) \<or>
+        (py\<^sub>1 < px\<^sub>1 \<and> px\<^sub>1 < px\<^sub>2 \<and> px\<^sub>2 < py\<^sub>2)"
+    using `px\<^sub>1 < px\<^sub>2` and `py\<^sub>1 < py\<^sub>2` and `px\<^sub>1 \<noteq> py\<^sub>1` and `px\<^sub>2 \<noteq> py\<^sub>2` and `px\<^sub>1 \<noteq> py\<^sub>2` and `px\<^sub>2 \<noteq> py\<^sub>1`
+      by (metis linorder_cases)
+
+  moreover have "?this \<Longrightarrow> ?thesis"
+  proof (erule rev_mp, simp only: disj_assoc[symmetric], intro impI, (erule disjE)+)
+    assume "px\<^sub>1 < px\<^sub>2 \<and> px\<^sub>2 < py\<^sub>1 \<and> py\<^sub>1 < py\<^sub>2"
+
+    thm interleave_left_lappend[where xs = xs and ys = "x\<^sub>1 # x\<^sub>2 # xs'" and t = t and zs = "ys \<frown> (y\<^sub>1 # y\<^sub>2 # ys')"]
+
+(*
+    have step1: "?lhs =
+      (xs \<triangleright> ltakeLeft (llength xs) t \<triangleleft> \<up> (llength (\<rr> (ltakeLeft (llength xs) t))) (ys \<frown> (y\<^sub>1 # y\<^sub>2 # ys'))) \<frown>
+      (x\<^sub>1 # x\<^sub>2 # xs' \<triangleright> ldropLeft (llength xs) t \<triangleleft> \<down> (llength (\<rr> (ltakeLeft (llength xs) t))) (ys \<frown> (y\<^sub>1 # y\<^sub>2 # ys')))"
+      apply (rule interleave_left_lappend[where xs = xs and ys = "x\<^sub>1 # x\<^sub>2 # xs'" and t = t and zs = "ys \<frown> (y\<^sub>1 # y\<^sub>2 # ys')"])
+      apply (rule assms(1))
+      by (rule assms(2))
+
+    have step2: "... =
+      (xs \<triangleright> ltakeLeft (llength xs) t \<triangleleft> \<up> (llength (\<rr> (ltakeLeft (llength xs) t))) (ys \<frown> (y\<^sub>1 # y\<^sub>2 # ys'))) \<frown>
+      (Inl x\<^sub>1 # LNil) \<frown>
+      (x\<^sub>2 # xs' \<triangleright> ltl (ldropLeft (llength xs) t) \<triangleleft> \<down> (llength (\<rr> (ltakeLeft (llength xs) t))) (ys \<frown> (y\<^sub>1 # y\<^sub>2 # ys')))"
+      sorry
+
+    have step3: "... =
+      (xs \<triangleright> ltakeLeft (llength xs) t \<triangleleft> \<up> (llength (\<rr> (ltakeLeft (llength xs) t))) ys) \<frown>
+      (Inl x\<^sub>1 # LNil) \<frown>
+      (x\<^sub>2 # xs' \<triangleright> ltl (ldropLeft (llength xs) t) \<triangleleft> \<down> (llength (\<rr> (ltakeLeft (llength xs) t))) ys \<frown> (y\<^sub>1 # y\<^sub>2 # ys'))"
+      sorry
+
+    have step4: "... =
+      (xs \<triangleright> ltakeLeft (llength xs) t \<triangleleft> \<up> (llength (\<rr> (ltakeLeft (llength xs) t))) ys) \<frown>
+      (Inl x\<^sub>1 # LNil) \<frown>
+      (LNil \<frown> (x\<^sub>2 # xs') \<triangleright> ltl (ldropLeft (llength xs) t) \<triangleleft> \<down> (llength (\<rr> (ltakeLeft (llength xs) t))) ys \<frown> (y\<^sub>1 # y\<^sub>2 # ys'))"
+      by (metis lappend_code(1))
+
+    have step5: "... =
+      (xs \<triangleright> ltakeLeft (llength xs) t \<triangleleft> \<up> (llength (\<rr> (ltakeLeft (llength xs) t))) ys) \<frown>
+      (Inl x\<^sub>1 # LNil) \<frown>
+      (LNil \<triangleright> ltakeLeft 0 (ltl (ldropLeft (llength xs) t)) \<triangleleft> \<up> (llength (\<rr> (ltakeLeft 0 (ltl (ldropLeft (llength xs) t))))) (\<down> (llength (\<rr> (ltakeLeft (llength xs) t))) ys \<frown> (y\<^sub>1 # y\<^sub>2 # ys'))) \<frown>
+      (x\<^sub>2 # xs' \<triangleright> ldropLeft 0 (ltl (ldropLeft (llength xs) t)) \<triangleleft> \<down> (llength (\<rr> (ltakeLeft 0 (ltl (ldropLeft (llength xs) t))))) (\<down> (llength (\<rr> (ltakeLeft (llength xs) t))) ys \<frown> (y\<^sub>1 # y\<^sub>2 # ys')))"
+      apply (subst interleave_left_lappend)
+      prefer 3
+      apply simp
+      apply (metis lappend_assoc)
+      sorry
+
+    have step6: "... =
+      (xs \<triangleright> ltakeLeft (llength xs) t \<triangleleft> \<up> (llength (\<rr> (ltakeLeft (llength xs) t))) ys) \<frown>
+      (Inl x\<^sub>1 # LNil) \<frown>
+      (LNil \<triangleright> ltakeLeft 0 (ltl (ldropLeft (llength xs) t)) \<triangleleft> \<up> (llength (\<rr> (ltakeLeft 0 (ltl (ldropLeft (llength xs) t))))) (\<down> (llength (\<rr> (ltakeLeft (llength xs) t))) ys \<frown> (y\<^sub>1 # y\<^sub>2 # ys'))) \<frown>
+      (Inl x\<^sub>2 # LNil) \<frown>
+      (xs' \<triangleright> ltl (ldropLeft 0 (ltl (ldropLeft (llength xs) t))) \<triangleleft> \<down> (llength (\<rr> (ltakeLeft 0 (ltl (ldropLeft (llength xs) t))))) (\<down> (llength (\<rr> (ltakeLeft (llength xs) t))) ys \<frown> (y\<^sub>1 # y\<^sub>2 # ys')))"
+      sorry
+
+    have step7: "... =
+      (xs \<triangleright> ltakeLeft (llength xs) t \<triangleleft> \<up> (llength (\<rr> (ltakeLeft (llength xs) t))) ys) \<frown>
+      (Inl x\<^sub>1 # LNil) \<frown>
+      lmap Inr (\<up> (llength (\<rr> (ltakeLeft 0 (ltl (ldropLeft (llength xs) t))))) (\<down> (llength (\<rr> (ltakeLeft (llength xs) t))) ys)) \<frown>
+      (Inl x\<^sub>2 # LNil) \<frown>
+      (xs' \<triangleright> ltl (ldropLeft 0 (ltl (ldropLeft (llength xs) t))) \<triangleleft> \<down> (llength (\<rr> (ltakeLeft 0 (ltl (ldropLeft (llength xs) t))))) (\<down> (llength (\<rr> (ltakeLeft (llength xs) t))) ys) \<frown> (y\<^sub>1 # y\<^sub>2 # ys'))"
+      sorry
+
+    have "\<up> (llength (\<rr> (ltakeLeft (llength xs) t))) (ys \<frown> (y\<^sub>1 # y\<^sub>2 # ys')) = \<up> (llength (\<rr> (ltakeLeft (llength xs) t))) ys"
+      apply (subst ltake_lappend_llength)
+      apply simp
+      thm py\<^sub>1_def
+*)
+
+    thus ?thesis
+      sorry
+  next
+    assume "px\<^sub>1 < py\<^sub>1 \<and> py\<^sub>1 < px\<^sub>2 \<and> px\<^sub>2 < py\<^sub>2"
+    thus ?thesis
+      sorry
+  next
+    assume "px\<^sub>1 < py\<^sub>1 \<and> py\<^sub>1 < py\<^sub>2 \<and> py\<^sub>2 < px\<^sub>2"
+    thus ?thesis
+      sorry
+  next
+    assume "py\<^sub>1 < py\<^sub>2 \<and> py\<^sub>2 < px\<^sub>1 \<and> px\<^sub>1 < px\<^sub>2"
+    thus ?thesis
+      sorry
+  next
+    assume "py\<^sub>1 < px\<^sub>1 \<and> px\<^sub>1 < py\<^sub>2 \<and> py\<^sub>2 < px\<^sub>2"
+    thus ?thesis
+      sorry
+  next
+    assume "py\<^sub>1 < px\<^sub>1 \<and> px\<^sub>1 < px\<^sub>2 \<and> px\<^sub>2 < py\<^sub>2"
+    thus ?thesis
+      sorry
+  qed
+  ultimately show "?thesis"
+    by blast
+qed
+
+(* ################################## Environments ################################## *)
+
+coinductive env :: "'a rel \<Rightarrow> ('a \<times> 'a) llist \<Rightarrow> bool" for "R" where
+  EqNil [intro!,simp]: "env R LNil"
+| EqSingle [intro!,simp]: "env R (LCons \<sigma> LNil)"
+| EqPair [intro!]: "(snd \<sigma>, fst \<sigma>') \<in> R \<Longrightarrow> env R (LCons \<sigma>' t) \<Longrightarrow> env R (LCons \<sigma> (LCons \<sigma>' t))"
+
+definition Env :: "'a rel \<Rightarrow> ('a \<times> 'a) lan \<Rightarrow> ('a \<times> 'a) lan" (infixr "\<Colon>" 52) where
+  "R \<Colon> X \<equiv> X \<inter> Collect (env (R\<^sup>*))"
+
+lemma env_tl [dest]: "env R (LCons \<sigma> t) \<Longrightarrow> env R t"
+  by (erule env.cases) auto
+
+lemma env_LConsD [dest]: "env R (LCons \<sigma> (LCons \<sigma>' t)) \<Longrightarrow> (snd \<sigma>, fst \<sigma>') \<in> R"
+  by (erule env.cases) auto
+
+lemma env_interE1 [elim]: "env (R \<inter> S) x \<Longrightarrow> env S x"
+proof -
+  assume "env (R \<inter> S) x"
+  thus ?thesis
+  proof coinduct
+    case (env t)
+    show ?case
+    proof (cases t)
+      assume "t = LNil"
+      thus ?case
+        by simp
+    next
+      fix \<sigma> t'
+      assume [simp]: "t = LCons \<sigma> t'"
+      hence "?EqSingle \<or> ?EqPair"
+      proof (cases t')
+        assume "t' = LNil"
+        thus "?EqSingle \<or> ?EqPair" by simp
+      next
+        fix \<sigma>' t''
+        assume [simp]: "t' = LCons \<sigma>' t''"
+        from env
+        have "?EqPair"
+          by auto
+        thus "?EqSingle \<or> ?EqPair" by simp
+      qed
+      thus ?case by simp
+    qed
+  qed
+qed
+
+lemma env_interE2 [elim]: "env (R \<inter> S) x \<Longrightarrow> env R x"
+  by (metis env_interE1 inf_commute)
+
+lemma env_InterE: "env (\<Inter>\<RR>) x \<Longrightarrow> R \<in> \<RR> \<Longrightarrow> env R x"
+proof -
+  assume "env (\<Inter>\<RR>) x" and "R \<in> \<RR>"
+  hence "env (\<Inter>\<RR>) x \<and> R \<in> \<RR>" by simp
+  thus "env R x"
+  proof coinduct
+    case (env t)
+    thus ?case
+    proof (cases t)
+      assume "t = LNil"
+      thus ?case
+        by simp
+    next
+      fix \<sigma> t'
+      assume [simp]: "t = LCons \<sigma> t'"
+      hence "?EqSingle \<or> ?EqPair"
+      proof (cases t')
+        assume "t' = LNil"
+        thus "?EqSingle \<or> ?EqPair" by simp
+      next
+        fix \<sigma>' t''
+        assume [simp]: "t' = LCons \<sigma>' t''"
+        from env
+        have "?EqPair"
+          by auto
+        thus "?EqSingle \<or> ?EqPair"
+          by auto
+      qed
+      thus ?case by simp
+    qed
+  qed
+qed
+
+lemma env_InterE_star: "env ((\<Inter>{R\<^sup>* |R. R \<in> \<RR>})\<^sup>*) x \<Longrightarrow> R \<in> \<RR> \<Longrightarrow> env (R\<^sup>*) x"
+proof -
+  assume "env ((\<Inter>{R\<^sup>* |R. R \<in> \<RR>})\<^sup>*) x" and "R \<in> \<RR>"
+  hence "env ((\<Inter>{R\<^sup>* |R. R \<in> \<RR>})\<^sup>*) x \<and> R \<in> \<RR>" by simp
+  thus "env (R\<^sup>*) x"
+  proof coinduct
+    case (env t)
+    thus ?case
+    proof (cases t)
+      assume "t = LNil"
+      thus ?case
+        by simp
+    next
+      fix \<sigma> t'
+      assume [simp]: "t = LCons \<sigma> t'"
+      hence "?EqSingle \<or> ?EqPair"
+      proof (cases t')
+        assume "t' = LNil"
+        thus "?EqSingle \<or> ?EqPair" by simp
+      next
+        fix \<sigma>' t''
+        assume [simp]: "t' = LCons \<sigma>' t''"
+        from env
+        have "?EqPair"
+          apply auto
+          apply (drule env_LConsD)
+          apply (erule set_rev_mp)
+          apply (subst rtrancl_idemp[symmetric]) back back
+          apply (rule rtrancl_mono)
+          by auto
+        thus "?EqSingle \<or> ?EqPair"
+          by auto
+      qed
+      thus ?case by simp
+    qed
+  qed
+qed
+
+lemma env_interI [intro]: "env R t \<Longrightarrow> env S t \<Longrightarrow> env (R \<inter> S) t"
+proof -
+  assume "env R t" and "env S t"
+  hence "env R t \<and> env S t"
+    by auto
+  thus "env (R \<inter> S) t"
+  proof (coinduct)
+    case (env t)
+    thus ?case
+    proof (cases t)
+      assume "t = LNil"
+      thus ?case
+        by simp
+    next
+      fix \<sigma> t'
+      assume [simp]: "t = LCons \<sigma> t'"
+      hence "?EqSingle \<or> ?EqPair"
+      proof (cases t')
+        assume "t' = LNil"
+        thus "?EqSingle \<or> ?EqPair" by simp
+      next
+        fix \<sigma>' t''
+        assume [simp]: "t' = LCons \<sigma>' t''"
+        from env
+        show "?EqSingle \<or> ?EqPair"
+          by auto
+      qed
+      thus ?case by simp
+    qed
+  qed
+qed
+
+lemma env_InterI [intro]: "(\<And>R. R \<in> \<RR> \<Longrightarrow> env R t) \<Longrightarrow> env (\<Inter>\<RR>) t"
+proof -
+  assume "(\<And>R. R \<in> \<RR> \<Longrightarrow> env R t)"
+  hence "(\<forall>R. R \<in> \<RR> \<longrightarrow> env R t)"
+    by auto
+  thus "env (\<Inter>\<RR>) t"
+  proof (coinduct)
+    case (env t)
+    thus ?case
+    proof (cases t)
+      assume "t = LNil"
+      thus ?case
+        by simp
+    next
+      fix \<sigma> t'
+      assume [simp]: "t = LCons \<sigma> t'"
+      hence "?EqSingle \<or> ?EqPair"
+      proof (cases t')
+        assume "t' = LNil"
+        thus "?EqSingle \<or> ?EqPair" by simp
+      next
+        fix \<sigma>' t''
+        assume [simp]: "t' = LCons \<sigma>' t''"
+        from env
+        show "?EqSingle \<or> ?EqPair"
+          by auto
+      qed
+      thus ?case by simp
+    qed
+  qed
+qed
+
+lemma contrp: "(\<not> P \<longrightarrow> Q) \<longleftrightarrow> (\<not> Q \<longrightarrow> P)"
+  by blast
+
+lemma environment_var': "\<not> env R xs \<longrightarrow> (\<exists>ys \<sigma> \<sigma>' zs. lfinite ys \<and> env R (ys \<frown> LCons \<sigma> LNil) \<and> xs = ys \<frown> LCons \<sigma> (LCons \<sigma>' zs) \<and> (snd \<sigma>, fst \<sigma>') \<notin> R)"
+proof (subst contrp, auto)
+  assume "\<forall>ys. lfinite ys \<longrightarrow>
+               (\<forall>a b. env R (ys \<frown> LCons (a, b) LNil) \<longrightarrow>
+                      (\<forall>a'. (\<forall>b' zs. xs \<noteq> ys \<frown> LCons (a, b) (LCons (a', b') zs)) \<or> (b, a') \<in> R))"
+  thus "env R xs"
+  proof coinduct
+    case (env t)
+    thus ?case
+    proof (cases t)
+      assume "t = LNil"
+      thus ?case
+        by simp
+    next
+      fix \<sigma> t'
+      assume [simp]: "t = LCons \<sigma> t'"
+      hence "?EqSingle \<or> ?EqPair"
+      proof (cases t')
+        assume "t' = LNil"
+        thus "?EqSingle \<or> ?EqPair" by simp
+      next
+        fix \<sigma>' t''
+        assume [simp]: "t' = LCons \<sigma>' t''"
+        from env
+        have "?EqPair"
+          apply (rule_tac x = \<sigma> in exI)
+          apply (rule_tac x = \<sigma>' in exI)
+          apply (rule_tac x = t'' in exI)
+          apply (intro conjI)
+          apply simp
+          apply simp
+          apply (erule_tac x = LNil in allE)
+          apply simp
+          apply (metis surjective_pairing)
+          apply (subgoal_tac "(snd \<sigma>, fst \<sigma>') \<in> R")
+          defer
+          apply simp
+          apply (erule_tac x = LNil in allE)
+          apply simp
+          apply (metis surjective_pairing)
+          apply auto
+          apply (erule_tac x = "LCons \<sigma> ys" in allE)
+          apply (erule impE)
+          apply simp
+          apply (erule_tac x = a in allE)
+          apply (erule_tac x = b in allE)
+          apply (erule impE)
+          apply simp
+          apply (subgoal_tac "(\<exists>\<sigma>'' ys'. ys = LCons \<sigma>'' ys') \<or> ys = LNil")
+          apply (erule disjE)
+          apply (erule exE)+
+          apply simp
+          apply (metis env.EqPair)
+          apply simp
+          apply (metis EqPair EqSingle fst_conv)
+          apply (metis neq_LNil_conv)
+          apply (erule_tac x = a' in allE)
+          apply (erule disjE)
+          apply (metis lappend_code(2))
+          by blast
+        thus "?EqSingle \<or> ?EqPair"
+          by auto
+      qed
+      thus ?case by simp
+    qed
+  qed
+qed
+
+lemma environment_var: "\<not> env R xs \<Longrightarrow> (\<exists>ys \<sigma> \<sigma>' zs. lfinite ys \<and> env R (ys \<frown> LCons \<sigma> LNil) \<and> xs = ys \<frown> LCons \<sigma> (LCons \<sigma>' zs) \<and> (snd \<sigma>, fst \<sigma>') \<notin> R)"
+  by (metis environment_var')
+
+lemma environment': "\<not> env R xs \<longrightarrow> (\<exists>ys \<sigma> \<sigma>' zs. lfinite ys \<and> xs = ys \<frown> LCons \<sigma> (LCons \<sigma>' zs) \<and> (snd \<sigma>, fst \<sigma>') \<notin> R)"
+proof (subst contrp, auto)
+  assume "\<forall>ys. lfinite ys \<longrightarrow> (\<forall>a b a'. (\<forall>b' zs. xs \<noteq> ys \<frown> LCons (a, b) (LCons (a', b') zs)) \<or> (b, a') \<in> R)"
+  thus "env R xs"
+  proof coinduct
+    case (env t)
+    thus ?case
+    proof (cases t)
+      assume "t = LNil"
+      thus ?case
+        by simp
+    next
+      fix \<sigma> t'
+      assume [simp]: "t = LCons \<sigma> t'"
+      hence "?EqSingle \<or> ?EqPair"
+      proof (cases t')
+        assume "t' = LNil"
+        thus "?EqSingle \<or> ?EqPair" by simp
+      next
+        fix \<sigma>' t''
+        assume [simp]: "t' = LCons \<sigma>' t''"
+        from env
+        have "?EqPair"
+          apply auto
+          apply (metis lappend_code(1) lfinite_code(1) surjective_pairing)
+          by (metis lappend_code(2) lfinite_LCons)
+        thus "?EqSingle \<or> ?EqPair"
+          by auto
+      qed
+      thus ?case by simp
+    qed
+  qed
+qed
+
+lemma environment: "\<not> env R xs \<Longrightarrow> (\<exists>ys \<sigma> \<sigma>' zs. lfinite ys \<and> xs = ys \<frown> LCons \<sigma> (LCons \<sigma>' zs) \<and> (snd \<sigma>, fst \<sigma>') \<notin> R)"
+  by (metis environment')
+
+lemma LCons_lappend_LNil: "LCons y ys = LCons y LNil \<frown> ys"
+  by (metis lappend_code(1) lappend_code(2))
+
+lemma gap_environment: "lfinite xs \<Longrightarrow> env R (LCons \<sigma> LNil \<frown> xs \<frown> LCons \<sigma>' LNil) \<Longrightarrow> (snd \<sigma>, fst \<sigma>') \<in> (R \<union> lset xs)\<^sup>*"
+proof (induct arbitrary: \<sigma> rule: lfinite.induct)
+  case lfinite_LNil thus ?case
+    by simp (metis env_LConsD r_into_rtrancl)
+next
+  case (lfinite_LConsI xs x)
+  hence "env R (LCons \<sigma> (LCons x (xs \<frown> LCons \<sigma>' LNil)))"
+    by (metis LCons_lappend_LNil lappend_code(2))
+  hence "env R (LCons x (xs \<frown> LCons \<sigma>' LNil))" and "(snd \<sigma>, fst x) \<in> R"
+    by - (metis env_tl, metis env_LConsD)
+  hence "env R (LCons x LNil \<frown> xs \<frown> LCons \<sigma>' LNil)"
+    by (metis LCons_lappend_LNil lappend_code(2))
+  hence "(snd x, fst \<sigma>') \<in> (R \<union> lset xs)\<^sup>*"
+    by (metis lfinite_LConsI.hyps(2))
+  hence "(snd x, fst \<sigma>') \<in> (R \<union> lset (LCons x xs))\<^sup>*"
+    by (rule set_rev_mp) (auto intro!: rtrancl_mono)
+  moreover have "(fst x, snd x) \<in> lset (LCons x xs)"
+    by (metis lset_intros(1) surjective_pairing)
+  ultimately show ?case using `(snd \<sigma>, fst x) \<in> R`
+    apply -
+    apply (rule converse_rtrancl_into_rtrancl[where b = "fst x"])
+    apply simp
+    apply (rule converse_rtrancl_into_rtrancl[where b = "snd x"])
+    by simp_all
+qed
+
+lemma shuffle_interleaving: "zs \<in> xs \<sha> ys \<Longrightarrow> zs = xs \<triangleright> traj zs \<triangleleft> ys"
+  by (auto simp add: tshuffle_words_def reinterleave)
+
+lemma shuffle_env_left:
+  assumes "zs \<in> xs \<sha> ys"
+  and "env R (lmap \<langle>id,id\<rangle> zs)"
+  shows "env ((R \<union> lset ys)\<^sup>*) xs"
+proof (rule classical)
+  assume "\<not> env ((R \<union> lset ys)\<^sup>*) xs"
+  hence "\<exists>as \<sigma> \<sigma>' bs. lfinite as \<and> xs = as \<frown> LCons \<sigma> (LCons \<sigma>' bs) \<and> (snd \<sigma>, fst \<sigma>') \<notin> (R \<union> lset ys)\<^sup>*"
+    by (metis environment)
+  then obtain as and \<sigma> and \<sigma>' and bs
+  where lfinite_as: "lfinite as" and xs_split: "xs = as \<frown> LCons \<sigma> (LCons \<sigma>' bs)" and "(snd \<sigma>, fst \<sigma>') \<notin> (R \<union> lset ys)\<^sup>*"
+    by auto
+
+  from assms(1)
+  have zs_llen: "llength (\<ll> zs) = llength xs"
+    by (auto simp add: tshuffle_words_def)
+
+  have zs_interleave: "zs = as \<frown> LCons \<sigma> (LCons \<sigma>' bs) \<triangleright> traj zs \<triangleleft> ys"
+    by (metis assms(1) shuffle_interleaving xs_split)
+  have traj_zs_llen: "llength (\<ll> (traj zs)) = llength as + llength (LCons \<sigma> (LCons \<sigma>' bs))"
+    by (simp add: zs_llen xs_split)
+  have traj_zs_rlen: "llength (\<rr> (traj zs)) = llength ys"
+    using assms(1) by (simp add: tshuffle_words_def) 
+
+  from interleave_left_lappend[OF lfinite_as zs_interleave traj_zs_llen traj_zs_rlen]
+  obtain ys' and ys''
+  where "lfinite ys'" and ys_split: "ys = ys' \<frown> ys''"
+  and zs_prefix: "zs = (as \<triangleright> \<up> (llength as + llength ys') (traj zs) \<triangleleft> ys') \<frown> (LCons \<sigma> (LCons \<sigma>' bs) \<triangleright> LCons (Inl ()) (\<down> (eSuc (llength as + llength ys')) (traj zs)) \<triangleleft> ys'')"
+    by auto
+
+  let ?prefix = "as \<triangleright> \<up> (llength as + llength ys') (traj zs) \<triangleleft> ys'"
+  let ?t = "\<down> (eSuc (llength as + llength ys')) (traj zs)"
+
+  have "zs = ?prefix \<frown> (LCons \<sigma> (LCons \<sigma>' bs) \<triangleright> LCons (Inl ()) ?t \<triangleleft> ys'')"
+    by (metis zs_prefix)
+  also have "... = ?prefix \<frown> LCons (Inl \<sigma>) (LCons \<sigma>' bs \<triangleright> ?t \<triangleleft> ys'')"
+    by (metis zs_prefix interleave_left lhd_LCons ltl_simps(2))
+  also have "... = ?prefix \<frown> LCons (Inl \<sigma>) (LCons \<sigma>' bs \<triangleright> ltakeWhile is_right ?t \<frown> LCons (Inl ()) (ltl (ldropWhile is_right ?t)) \<triangleleft> ys'')"
+    sorry
+  also have "... = ?prefix \<frown> LCons (Inl \<sigma>) LNil \<frown> lmap Inr (\<up> (llength (ltakeWhile is_right ?t)) ys'') \<frown> LCons (Inl \<sigma>') (bs \<triangleright> ltl (ldropWhile is_right ?t) \<triangleleft> \<down> (llength (ltakeWhile is_right ?t)) ys'')"
+    sorry
+  finally have "zs = ?prefix \<frown> LCons (Inl \<sigma>) LNil \<frown> lmap Inr (\<up> (llength (ltakeWhile is_right ?t)) ys'') \<frown> LCons (Inl \<sigma>') (bs \<triangleright> ltl (ldropWhile is_right ?t) \<triangleleft> \<down> (llength (ltakeWhile is_right ?t)) ys'')"
+    by simp
+
+  hence "env R (LCons \<sigma> LNil \<frown> \<up> (llength (ltakeWhile is_right ?t)) ys'' \<frown> LCons \<sigma>' LNil)"
+    sorry  
+  hence "(snd \<sigma>, fst \<sigma>') \<in> (R \<union> lset (\<up> (llength (ltakeWhile is_right ?t)) ys''))\<^sup>*"
+    apply -
+    apply (erule gap_environment[rotated 1])
+    defer
+    apply (rule lfinite_ltake_llength)
+    sorry
+  hence "(snd \<sigma>, fst \<sigma>') \<in> (R \<union> lset ys)\<^sup>*"
+    apply (rule set_rev_mp)
+    apply (intro rtrancl_mono Un_mono order_refl)
+    by (metis Un_upper2 `lfinite ys'` lset_lappend_lfinite lset_ltake order.trans ys_split)
+  from this and `(snd \<sigma>, fst \<sigma>') \<notin> (R \<union> lset ys)\<^sup>*` have False
+    by blast
+  thus ?thesis by blast
+qed
+
+lemma shuffle_env_right:
+  assumes "zs \<in> xs \<sha> ys"
+  and "env R (lmap \<langle>id,id\<rangle> zs)"
+  shows "env ((R \<union> lset xs)\<^sup>*) ys"
+  sorry
+
+lemma env_lappend1: "env R (xs \<frown> ys) \<Longrightarrow> env R xs"
+  sorry
+
+lemma env_lappend2: "lfinite xs \<Longrightarrow> env R (xs \<frown> ys) \<Longrightarrow> env R ys"
+  sorry
+
+(* ################################## Rely guarantee ################################## *)
+
+lemma tshuffle_lappend: "lfinite zs\<^sub>1 \<Longrightarrow> zs\<^sub>1 \<in> xs\<^sub>1 \<sha> ys\<^sub>1 \<Longrightarrow> zs\<^sub>2 \<in> xs\<^sub>2 \<sha> ys\<^sub>2 \<Longrightarrow> zs\<^sub>1 \<frown> zs\<^sub>2 \<in> (xs\<^sub>1 \<frown> xs\<^sub>2) \<sha> (ys\<^sub>1 \<frown> ys\<^sub>2)"
+  by (auto simp add: tshuffle_words_def lefts_append rights_append)
+
+lemma tshuffle_left_LCons: "zs \<in> xs \<sha> ys \<Longrightarrow> Inl z # zs \<in> (z # xs) \<sha> ys"
+  by (auto simp add: tshuffle_words_def)
+
+lemma llength_enat_lfinite: "\<exists>n. llength xs = enat n \<Longrightarrow> lfinite xs"
+  by (metis enat.distinct(1) not_lfinite_llength)
+
+lemma llength_interleave: "Valid xs t ys \<Longrightarrow> llength (xs \<triangleright> t \<triangleleft> ys) = llength xs + llength ys"
+  sorry
+
+definition rg'' :: "'a rel \<Rightarrow> ('a \<times> 'a) llist \<Rightarrow> ('a \<times> 'a) llist \<Rightarrow> bool" where
+  "rg'' R xs xs' \<equiv> (\<exists>xs\<^sub>p \<sigma>\<^sub>1 \<sigma>\<^sub>1' \<sigma>\<^sub>2 \<sigma>\<^sub>2' \<sigma>\<^sub>2'' as bs. xs = xs\<^sub>p \<frown> ((\<sigma>\<^sub>1, \<sigma>\<^sub>1') # (\<sigma>\<^sub>2, \<sigma>\<^sub>2') # as) \<and> xs' = xs\<^sub>p \<frown> ((\<sigma>\<^sub>1, \<sigma>\<^sub>1') # (\<sigma>\<^sub>2, \<sigma>\<^sub>2'') # bs) \<and> lfinite xs\<^sub>p \<and> (\<sigma>\<^sub>1', \<sigma>\<^sub>2) \<notin> R \<and> env R (xs\<^sub>p \<frown> ((\<sigma>\<^sub>1, \<sigma>\<^sub>1') # LNil)))"
+
+definition rg' :: "'a rel \<Rightarrow> ('a \<times> 'a) llist \<Rightarrow> ('a \<times> 'a) llist \<Rightarrow> bool" where
+  "rg' R xs xs' \<equiv> (\<exists>xs\<^sub>p \<sigma>\<^sub>1 \<sigma>\<^sub>1' \<sigma>\<^sub>2 \<sigma>\<^sub>2' \<sigma>\<^sub>2'' as bs. xs = xs\<^sub>p \<frown> ((\<sigma>\<^sub>1, \<sigma>\<^sub>1') # (\<sigma>\<^sub>2, \<sigma>\<^sub>2') # as) \<and> xs' = xs\<^sub>p \<frown> ((\<sigma>\<^sub>1, \<sigma>\<^sub>1') # (\<sigma>\<^sub>2, \<sigma>\<^sub>2'') # bs) \<and> lfinite xs\<^sub>p \<and> (\<sigma>\<^sub>1', \<sigma>\<^sub>2) \<notin> R)"
+
+lemma rg''_intro: "lfinite xs\<^sub>p \<Longrightarrow> (\<sigma>\<^sub>1', \<sigma>\<^sub>2) \<notin> R \<Longrightarrow>
+       rg'' R (xs\<^sub>p \<frown> ((\<sigma>\<^sub>1, \<sigma>\<^sub>1') # (\<sigma>\<^sub>2, \<sigma>\<^sub>2') # as)) (xs\<^sub>p \<frown> ((\<sigma>\<^sub>1, \<sigma>\<^sub>1') # (\<sigma>\<^sub>2, \<sigma>\<^sub>2'') # bs))"
+  apply (induct rule: lfinite_induct)
+  apply (simp add: rg''_def)
+  apply (rule_tac x = LNil in exI)
+  apply simp
+  apply (subgoal_tac "\<exists>\<tau>\<^sub>1 \<tau>\<^sub>1'. x = (\<tau>\<^sub>1,\<tau>\<^sub>1')")
+  apply (erule exE)+
+  apply simp
+  prefer 2
+  apply (metis surj_pair)
+  apply (simp only: rg''_def)
+  apply (erule exE)+
+  apply (erule conjE)+
+  apply simp
+  apply (subgoal_tac "xs\<^sub>p = LNil \<or> (\<exists>\<tau>\<^sub>2 \<tau>\<^sub>2' xs\<^sub>p'. xs\<^sub>p = (\<tau>\<^sub>2, \<tau>\<^sub>2') # xs\<^sub>p')")
+  prefer 2
+  apply (metis llist.exhaust prod.exhaust)
+  apply (erule disjE)
+  apply simp
+  apply (subgoal_tac "(\<tau>\<^sub>1',\<sigma>\<^sub>1'') \<in> R \<or> (\<tau>\<^sub>1',\<sigma>\<^sub>1'') \<notin> R")
+  prefer 2
+  apply metis
+  apply (erule disjE)
+  apply (rule_tac x = "(\<tau>\<^sub>1, \<tau>\<^sub>1') # LNil" in exI)
+  apply (rule_tac x = \<sigma>\<^sub>1'' in exI, rule_tac x = \<sigma>\<^sub>1''' in exI, rule_tac x = \<sigma>\<^sub>2''' in exI)
+  apply (intro conjI)
+  apply simp
+  apply simp
+  apply simp
+  apply simp
+  apply simp
+  apply (metis EqPair EqSingle fst_conv snd_conv)
+  apply (rule_tac x = "LNil" in exI)
+  apply (rule_tac x = \<tau>\<^sub>1 in exI, rule_tac x = \<tau>\<^sub>1' in exI, rule_tac x = \<sigma>\<^sub>1'' in exI)
+  apply (intro conjI)
+  apply simp
+  apply simp
+  apply simp
+  apply simp
+  apply simp
+  apply (erule exE)+
+  apply simp
+  apply (subgoal_tac "(\<tau>\<^sub>1',\<tau>\<^sub>2) \<in> R \<or> (\<tau>\<^sub>1',\<tau>\<^sub>2) \<notin> R")
+  apply (erule disjE)
+  apply (rule_tac x = "(\<tau>\<^sub>1, \<tau>\<^sub>1') # (\<tau>\<^sub>2, \<tau>\<^sub>2') # xs\<^sub>p'" in exI)
+  apply (rule_tac x = \<sigma>\<^sub>1'' in exI, rule_tac x = \<sigma>\<^sub>1''' in exI, rule_tac x = \<sigma>\<^sub>2''' in exI)
+  apply (intro conjI)
+  apply simp
+  apply blast
+  apply simp
+  apply blast
+  apply simp
+  apply simp
+  apply simp
+  apply (metis EqPair fst_conv snd_conv)
+  prefer 2
+  apply metis
+  apply (rule_tac x = "LNil" in exI)
+  apply (rule_tac x = \<tau>\<^sub>1 in exI, rule_tac x = \<tau>\<^sub>1' in exI, rule_tac x = \<tau>\<^sub>2 in exI)
+  apply (intro conjI)
+  by simp_all
+
+lemma rg''_is_rg': "rg'' R xs xs' \<longleftrightarrow> rg' R xs xs'"
+  apply default
+  apply (simp add: rg''_def rg'_def)
+  apply blast
+  apply (simp add: rg'_def)
+  apply (erule exE)+
+  apply (erule conjE)+
+  apply (erule exE)+
+  apply simp
+  apply (rule rg''_intro)
+  by auto
+
+axiomatization
+  alternate :: "'a llist \<Rightarrow> 'b llist \<Rightarrow> ('a + 'b) llist"
+where
+  alternate_prop: "alternate xs ys \<in> xs \<sha> ys"
+
+lemma
+  assumes "zs' \<in> xs' \<sha> ys'"
+  and "rg' ((R \<union> G\<^sub>2)\<^sup>*) xs xs'" and "lset xs \<subseteq> G\<^sub>1\<^sup>*"
+  and "rg' ((R \<union> G\<^sub>1)\<^sup>*) ys ys'" and "lset ys \<subseteq> G\<^sub>2\<^sup>*"
+  shows "\<exists>zs \<in> xs \<sha> ys. rg' (R\<^sup>*) (lmap \<langle>id,id\<rangle> zs) (lmap \<langle>id,id\<rangle> zs')"
+proof -
+  obtain xs\<^sub>p \<sigma>\<^sub>1 \<sigma>\<^sub>1' \<sigma>\<^sub>2 \<sigma>\<^sub>2' \<sigma>\<^sub>2'' xs\<^sub>t xs\<^sub>t'
+  where xs_def: "xs = xs\<^sub>p \<frown> ((\<sigma>\<^sub>1, \<sigma>\<^sub>1') # (\<sigma>\<^sub>2, \<sigma>\<^sub>2') # xs\<^sub>t)"
+  and xs'_def: "xs' = xs\<^sub>p \<frown> ((\<sigma>\<^sub>1, \<sigma>\<^sub>1') # (\<sigma>\<^sub>2, \<sigma>\<^sub>2'') # xs\<^sub>t')"
+  and lfinite_xs\<^sub>p: "lfinite xs\<^sub>p"
+  and "(\<sigma>\<^sub>1', \<sigma>\<^sub>2) \<notin> (R \<union> G\<^sub>2)\<^sup>*"
+  and "env ((R \<union> G\<^sub>2)\<^sup>*) (xs\<^sub>p \<frown> ((\<sigma>\<^sub>1, \<sigma>\<^sub>1') # LNil))"
+    sorry
+
+  obtain ys\<^sub>p \<tau>\<^sub>1 \<tau>\<^sub>1' \<tau>\<^sub>2 \<tau>\<^sub>2' \<tau>\<^sub>2'' ys\<^sub>t ys\<^sub>t'
+  where ys_def: "ys = ys\<^sub>p \<frown> ((\<tau>\<^sub>1, \<tau>\<^sub>1') # (\<tau>\<^sub>2, \<tau>\<^sub>2') # ys\<^sub>t)"
+  and ys'_def: "ys' = ys\<^sub>p \<frown> ((\<tau>\<^sub>1, \<tau>\<^sub>1') # (\<tau>\<^sub>2, \<tau>\<^sub>2'') # ys\<^sub>t')"
+  and lfinite_ys\<^sub>p: "lfinite ys\<^sub>p"
+  and "(\<tau>\<^sub>1', \<tau>\<^sub>2) \<notin> (R \<union> G\<^sub>1)\<^sup>*"
+  and "env ((R \<union> G\<^sub>2)\<^sup>*) (ys\<^sub>p \<frown> ((\<tau>\<^sub>1, \<tau>\<^sub>1') # LNil))"
+    sorry
+
+  def P \<equiv> "\<lambda>zs'. \<exists>zs \<in> xs \<sha> ys. rg' (R\<^sup>*) (lmap \<langle>id,id\<rangle> zs) (lmap \<langle>id,id\<rangle> zs')"
+
+  have "P (xs\<^sub>p \<frown> ((\<sigma>\<^sub>1, \<sigma>\<^sub>1') # (\<sigma>\<^sub>2, \<sigma>\<^sub>2'') # xs\<^sub>t') \<triangleright> traj zs' \<triangleleft> ys\<^sub>p \<frown> ((\<tau>\<^sub>1, \<tau>\<^sub>1') # (\<tau>\<^sub>2, \<tau>\<^sub>2'') # ys\<^sub>t'))"
+  proof (rule analyse_interleavings)
+    show "Valid (xs\<^sub>p \<frown> ((\<sigma>\<^sub>1, \<sigma>\<^sub>1') # (\<sigma>\<^sub>2, \<sigma>\<^sub>2'') # xs\<^sub>t')) (traj zs') (ys\<^sub>p \<frown> ((\<tau>\<^sub>1, \<tau>\<^sub>1') # (\<tau>\<^sub>2, \<tau>\<^sub>2'') # ys\<^sub>t'))"
+      using assms(1) by (simp add: Valid_def tshuffle_words_def xs'_def ys'_def)
+  next
+    show "lfinite xs\<^sub>p"
+      by (metis lfinite_xs\<^sub>p)
+  next
+    show "lfinite ys\<^sub>p"
+      by (metis lfinite_ys\<^sub>p)
+  next
+    fix xs\<^sub>1' xs\<^sub>2' xs\<^sub>3' t\<^sub>1 t\<^sub>2 t\<^sub>3 ys\<^sub>1 ys\<^sub>2 ys\<^sub>3
+    assume "Valid xs\<^sub>p t\<^sub>1 ys\<^sub>1" and "Valid xs\<^sub>1' t\<^sub>2 ys\<^sub>3" and "Valid xs\<^sub>3' t\<^sub>3 ys\<^sub>t'"
+    and "xs\<^sub>t' = xs\<^sub>1' \<frown> xs\<^sub>2' \<frown> xs\<^sub>3'"
+    and ys\<^sub>p_def: "ys\<^sub>p = ys\<^sub>1 \<frown> ys\<^sub>2 \<frown> ys\<^sub>3"
+
+    have "env ((R \<union> G\<^sub>2)\<^sup>*) ys\<^sub>p"
+      by (metis `env ((R \<union> G\<^sub>2)\<^sup>*) (ys\<^sub>p \<frown> ((\<tau>\<^sub>1, \<tau>\<^sub>1') # LNil))` env_lappend1)
+    have "env ((R \<union> G\<^sub>2)\<^sup>*) ys\<^sub>2"
+      by (metis `ys\<^sub>p = ys\<^sub>1 \<frown> ys\<^sub>2 \<frown> ys\<^sub>3` `env ((R \<union> G\<^sub>2)\<^sup>*) ys\<^sub>p` env_lappend1 env_lappend2 lfinite_lappend lfinite_ys\<^sub>p)
+
+    thus "P ((xs\<^sub>p \<triangleright> t\<^sub>1 \<triangleleft> ys\<^sub>1) \<frown> (Inl (\<sigma>\<^sub>1, \<sigma>\<^sub>1') # LNil) \<frown> lmap Inr ys\<^sub>2 \<frown> (Inl (\<sigma>\<^sub>2, \<sigma>\<^sub>2'') # LNil) \<frown>
+             (xs\<^sub>1' \<triangleright> t\<^sub>2 \<triangleleft> ys\<^sub>3) \<frown> (Inr (\<tau>\<^sub>1, \<tau>\<^sub>1') # LNil) \<frown> lmap Inl xs\<^sub>2' \<frown> (Inr (\<tau>\<^sub>2, \<tau>\<^sub>2'') # LNil) \<frown> (xs\<^sub>3' \<triangleright> t\<^sub>3 \<triangleleft> ys\<^sub>t'))"
+      proof (cases "ys\<^sub>2 = LNil")
+        assume [simp]: "ys\<^sub>2 = LNil"
+
+        show ?thesis
+          apply simp
+          apply (simp only: P_def)
+          apply (rule_tac x = "(xs\<^sub>p \<triangleright> t\<^sub>1 \<triangleleft> ys\<^sub>1) \<frown> (Inl (\<sigma>\<^sub>1, \<sigma>\<^sub>1') # LNil) \<frown> (Inl (\<sigma>\<^sub>2, \<sigma>\<^sub>2') # LNil) \<frown> alternate xs\<^sub>t (ys\<^sub>3 \<frown> ((\<tau>\<^sub>1, \<tau>\<^sub>1') # (\<tau>\<^sub>2, \<tau>\<^sub>2') # ys\<^sub>t))" in bexI)
+          prefer 2
+          apply (simp add: xs_def ys_def ys\<^sub>p_def lappend_assoc)
+          apply (rule tshuffle_lappend)
+          apply (rule llength_enat_lfinite)
+          apply (subst llength_interleave)
+          apply (metis `Valid xs\<^sub>p t\<^sub>1 ys\<^sub>1`)
+          apply (subst llength_lappend[symmetric])
+          apply (subgoal_tac "lfinite (xs\<^sub>p \<frown> ys\<^sub>1)")
+          apply (drule lfinite_llength_enat)
+          apply assumption
+          apply (metis lfinite_lappend lfinite_xs\<^sub>p lfinite_ys\<^sub>p ys\<^sub>p_def)
+          apply (metis `Valid xs\<^sub>p t\<^sub>1 ys\<^sub>1` shuffle_interleaving traj_to_shuffle)
+          apply (rule tshuffle_left_LCons)+
+          apply (rule alternate_prop)
+          apply (simp only: rg'_def)
+          apply (rule_tac x = "lmap \<langle>id,id\<rangle> (xs\<^sub>p \<triangleright> t\<^sub>1 \<triangleleft> ys\<^sub>1)" in exI)
+          apply (rule_tac x = \<sigma>\<^sub>1 in exI, rule_tac x = \<sigma>\<^sub>1' in exI)
+          apply (rule_tac x = \<sigma>\<^sub>2 in exI, rule_tac x = \<sigma>\<^sub>2' in exI, rule_tac x = \<sigma>\<^sub>2'' in exI)
+          apply (rule_tac x = "lmap \<langle>id,id\<rangle> (alternate xs\<^sub>t (ys\<^sub>3 \<frown> ((\<tau>\<^sub>1, \<tau>\<^sub>1') # (\<tau>\<^sub>2, \<tau>\<^sub>2') # ys\<^sub>t)))" in exI)
+          apply (rule_tac x = "lmap \<langle>id,id\<rangle> ((xs\<^sub>1' \<triangleright> t\<^sub>2 \<triangleleft> ys\<^sub>3) \<frown> (Inr (\<tau>\<^sub>1, \<tau>\<^sub>1') # LNil) \<frown> lmap Inl xs\<^sub>2' \<frown> (Inr (\<tau>\<^sub>2, \<tau>\<^sub>2'') # LNil) \<frown> (xs\<^sub>3' \<triangleright> t\<^sub>3 \<triangleleft> ys\<^sub>t'))" in exI)
+          apply (intro conjI)
+          apply (simp only: lmap_lappend_distrib llist.map(2))
+          apply simp
+          apply (metis LCons_lappend_LNil lappend_assoc)
+          apply (simp only: lmap_lappend_distrib llist.map(2))
+          apply simp
+          apply (metis LCons_lappend_LNil lappend_assoc)
+          apply (metis `Valid xs\<^sub>p t\<^sub>1 ys\<^sub>1` lfinite_lappend lfinite_lmap lfinite_shuffle lfinite_xs\<^sub>p lfinite_ys\<^sub>p shuffle_interleaving traj_to_shuffle ys\<^sub>p_def)  
+          by (metis `(\<sigma>\<^sub>1', \<sigma>\<^sub>2) \<notin> (R \<union> G\<^sub>2)\<^sup>*` in_rtrancl_UnI)
+  next
+    fix xs\<^sub>1' xs\<^sub>2' t\<^sub>1 t\<^sub>2 ys\<^sub>1 ys\<^sub>2
+    assume "Valid xs\<^sub>p t\<^sub>1 ys\<^sub>1"
+    and "Valid xs\<^sub>2' t\<^sub>2 ds"
+    and "bs = xs\<^sub>1' \<frown> xs\<^sub>2'"
+    and "ys\<^sub>p = ys\<^sub>1 \<frown> ys\<^sub>2"
+
+    thus "P ((xs\<^sub>p \<triangleright> t\<^sub>1 \<triangleleft> ys\<^sub>1) \<frown>
+             (Inl (\<sigma>\<^sub>1, \<sigma>\<^sub>1') # LNil) \<frown>
+             lmap Inr ys\<^sub>2 \<frown>
+             (Inr (\<tau>\<^sub>1, \<tau>\<^sub>1') # LNil) \<frown>
+             (Inl (\<sigma>\<^sub>2, \<sigma>\<^sub>2'') # LNil) \<frown>
+             lmap Inl xs\<^sub>1' \<frown>
+             (Inr (\<tau>\<^sub>2, \<tau>\<^sub>2'') # LNil) \<frown>
+             (xs\<^sub>2' \<triangleright> t\<^sub>2 \<triangleleft> ds))"
+      apply (simp only: P_def)
+      apply (simp only: rg'_def)
+      apply (rule_tac x = "(xs\<^sub>p \<triangleright> t\<^sub>1 \<triangleleft> ys\<^sub>1) \<frown> (Inl (\<sigma>\<^sub>1, \<sigma>\<^sub>1') # LNil) \<frown> lmap Inr ys\<^sub>2 \<frown> (Inr (\<tau>\<^sub>1, \<tau>\<^sub>1') # LNil) \<frown> (Inl (\<sigma>\<^sub>2, \<sigma>\<^sub>2') # LNil) \<frown> alternate as ((\<tau>\<^sub>2, \<tau>\<^sub>2'') # ds)" in bexI)
+      apply (simp only: rg'_def)
+      apply (rule_tac x = "lmap \<langle>id,id\<rangle> ((xs\<^sub>p \<triangleright> t\<^sub>1 \<triangleleft> ys\<^sub>1) \<frown> (Inl (\<sigma>\<^sub>1, \<sigma>\<^sub>1') # LNil) \<frown> lmap Inr ys\<^sub>2)" in exI)
+      apply (rule_tac x = \<tau>\<^sub>1 in exI) apply (rule_tac x = \<tau>\<^sub>1' in exI)
+      apply (rule_tac x = \<sigma>\<^sub>2 in exI) apply (rule_tac x = \<sigma>\<^sub>2' in exI)
+      apply (rule_tac x = \<sigma>\<^sub>2'' in exI)
+      apply (rule_tac x = "lmap \<langle>id,id\<rangle> (alternate as ((\<tau>\<^sub>2, \<tau>\<^sub>2'') # ds))" in exI)
+      apply (rule_tac x = "xs\<^sub>1' \<frown> ((\<tau>\<^sub>2, \<tau>\<^sub>2'') # LNil) \<frown> lmap \<langle>id,id\<rangle> (xs\<^sub>2' \<triangleright> t\<^sub>2 \<triangleleft> ds)" in exI)
+      apply (intro conjI)
+      
+      sledgehammer
 end
